Infrastructure.v
@@ -2,7 +2,6 @@ Require Import Lists.List. Import ListNotations.
 Require Import Strings.String.
 Require Import Logic.FunctionalExtensionality.
 Require Import Lia.
-From TLC Require Import LibLN.
 From LSEH Require Import Lexi.
 From LSEH Require Import Salt.
 From LSEH Require Import LexiToSalt.
@@ -55,75 +54,4 @@ Theorem heap_front_update : forall H a v1 v2,
 Proof with super_a.
   intros. unfold th_update. extensionality x. destruct (h_eqb a x)...
 Qed.
-(* ---------------------------------------------------------
-   ---- Helper Functions & Tactics for Locally Nameless ----
-   --------------------------------------------------------- *)
 
-Definition fv_val (v : L.value) : vars :=
-  match v with
-  | var_val (free_var x) => \{x}
-  | var_val (dbjind_var i) => \{}
-  | const_val c => \{}
-  end.
-Fixpoint fv_vlst (vlst : list L.value) : vars :=
-  match vlst with
-  | [] => \{}
-  | v :: vlst' => (fv_val v) \u (fv_vlst vlst')
-  end.
-Definition fv_exp (exp : L.expr) : vars :=
-  match exp with
-  | L.val_e val => fv_val val
-  | L.add val1 val2 =>
-      (fv_val val1) \u (fv_val val2)
-  | L.newref val_lst => fv_vlst val_lst
-  | L.pi _ val => fv_val val
-  | L.asgn val1 _ val2 =>
-      (fv_val val1) \u (fv_val val2)
-  | L.app val val_lst => (fv_val val) \u (fv_vlst val_lst)
-  | L.handle _ _ _ val => fv_val val
-  | L.raise _ val1 val2 =>
-      (fv_val val1) \u (fv_val val2)
-  | L.resume val1 val2 =>
-      (fv_val val1) \u (fv_val val2)
-  end.
-Fixpoint fv (tm : L.term) : vars :=
-  match tm with
-  | bind exp t => (fv_exp exp) \u (fv t)
-  | val_term v => (fv_val v)
-  | L.halt => \{}
-  end.
-(* ********************************************************************** *)
-(** ** Instantiation of tactics *)
-
-(** Tactic [gather_vars] returns a set of variables occurring in
-    the context of proofs, including domain of environments and
-    free variables in terms mentionned in the context. *)
-
-Ltac gather_vars :=
-  let A := gather_vars_with (fun x : vars => x) in
-  let B := gather_vars_with (fun x : var => \{x}) in
-  let C := gather_vars_with (fun x : L.value => fv_val x) in
-  let D := gather_vars_with (fun (x : list L.value) => fv_vlst x) in
-  let E := gather_vars_with (fun x : L.expr => fv_exp x) in
-  let F := gather_vars_with (fun x : L.term => fv x) in
-  constr:(A \u B \u C \u D \u E \u F).
-
-(** Tactic [pick_fresh x] adds to the context a new variable x
-    and a proof that it is fresh from all of the other variables
-    gathered by tactic [gather_vars]. *)
-
-Ltac pick_fresh Y :=
-  let L := gather_vars in (pick_fresh_gen L Y).
-
-(** Tactic [apply_fresh T as y] takes a lemma T of the form
-    [forall L ..., (forall x, x \notin L, P x) -> ... -> Q.]
-    instantiate L to be the set of variables occuring in the
-    context (by [gather_vars]), then introduces for the premise
-    with the cofinite quantification the name x as "y" (the second
-    parameter of the tactic), and the proof that x is not in L. *)
-
-Tactic Notation "apply_fresh" constr(T) "as" ident(x) :=
-  apply_fresh_base T gather_vars x.
-Tactic Notation "apply_fresh" constr(T) :=
-  apply_fresh_base T gather_vars ltac_no_arg.
-Hint Constructors lc_term L.step.
